

① let no. of signals amplified/sec be the states and x_n be the value of no. of signals amplified/sec after n sec.

Assuming Poisson's distribution and thus

$$P_{\lambda|x} = P(x|\lambda) = \frac{\lambda^x}{x!} \times e^{-\lambda}$$

where λ is no. of signals amplified in last sec. &

x is no. of signals amplified in next sec.

$$P_{0|0} = \frac{1^0}{0!} \times e^{-1}$$

$$P_{1|1} = \frac{1^1}{1!} \times e^{-1}$$

& similarly for others.

$$P_{2|2} = \frac{1^2}{2!} \times e^{-1}$$

⋮

$$P_{n|n} = \frac{1^n}{n!} \times e^{-1}$$

$$\sum_{i=0}^{\infty} P_{i|i} = 1$$

$P_{0|0} = 0$ since system stops at $n_u = 0$

Transition Matrix

2

$$A = \begin{matrix} & \begin{matrix} 0 & 1 & 2 & 3 & 4 & 5 & 6 & \dots & \infty \end{matrix} \\ \begin{matrix} 0 \\ 1 \\ 2 \\ 3 \\ 4 \\ 5 \\ 6 \\ \vdots \\ \infty \end{matrix} & \begin{bmatrix} 0 & 0 & 0 & 0 & 0 & 0 & 0 & \dots & \dots \\ e^{-1} & \frac{e^{-1}}{1!} & \frac{e^{-1}}{2!} & \frac{e^{-1}}{3!} & \frac{e^{-1}}{4!} & \frac{e^{-1}}{5!} & \frac{e^{-1}}{6!} & \dots & \dots \\ \frac{2^0 e^{-2}}{0!} & \frac{2^1 e^{-2}}{1!} & \frac{2^2 e^{-2}}{2!} & \frac{2^3 e^{-2}}{3!} & \frac{2^4 e^{-2}}{4!} & \frac{2^5 e^{-2}}{5!} & \frac{2^6 e^{-2}}{6!} & \dots & \dots \\ \vdots & \vdots & \vdots & \vdots & \vdots & \vdots & \vdots & \ddots & \ddots \end{bmatrix} \end{matrix}$$

So since the probability of ~~next~~ current state only depends upon the prev. state, it is a Markov model, with countably ∞ states for the problem.

2) let $P_{ij}^{(n)}$ be the probability of going from state i to j in n seconds.

so by Chapman - Kolmogorov Theorem

$$P_{ij}^{(n)} = \sum_k P_{ik}^{(r)} \times P_{kj}^{(n-r)}$$

$$\begin{aligned} P_{10}^{(2)} &= P_{10}^{(1)} \times P_{00}^{(1)} + P_{11}^{(1)} \times P_{10}^{(1)} \\ &+ \sum_{i=2}^{\infty} P_{1i}^{(1)} \times P_{i0}^{(1)} = A_{10}^2 \end{aligned}$$

$$\text{So } P_{ij}^n(n) = (A_{ij})^n$$

A is the transition matrix.

for Bogzora soon to stop, $j=0$ & $i=1$ since it starts with state 1.

$$E\left(\begin{smallmatrix} n \\ 0 \end{smallmatrix}\right) = \sum_{n=1}^{\infty} n \times P_{10}^n\left(\begin{smallmatrix} n \\ 0 \end{smallmatrix}\right)$$

$$= \sum_{n=1}^{\infty} n A_{10}^n$$

$$E(n) = 1 \times (A_{10}^1) + 2 \times (A_{10}^2) + 3(A_{10}^3) \dots + n A_{10}^n$$

$$= e^{-1} + 2e^{-1}(e^{-1} + S(0)) + 3\left(\sum_{i=1}^{\infty} A_{10}^2 A_{10}^i\right) \dots$$

$$E(n) = e^{-1} + 2e^{-1}(e^{-1} + S(0)) + 3 \sum_{i=1}^{\infty} \frac{e^{-1}}{i!} (S(i) + e^{-1}) \times e^{-i} \\ + \dots + n \sum_{i=1}^{\infty} A_{10}^{n-1} \times e^{-i}$$

⇒ Could not find a general term A_{10}^n calculations for

A_{10}^2 , A_{10}^3 are shown.

$$A_{1\alpha}^2 = \left(\sum_{i=2}^{\infty} A_{1i} \times A_{i\alpha} \right) + A_{11} A_{1\alpha} \quad \pm \quad \cancel{A_{10}} \quad \cancel{A_{0\alpha}}$$

for $\alpha=0$

$$A_{10}^2 = \sum_{i=2}^{\infty} \frac{e^{-1}}{i!} \times \frac{i^0 \times e^{-i}}{0!} + e^{-1} \times e^{-1} + \cancel{e^{-1} \times e^{-1}}$$

$$A_{10}^2 = \cancel{e^{-2}} + e^{-2} + e^{-1} (S(0))$$

$$S(x) = \sum_{k=2}^{\infty} \frac{k^x e^{-k}}{k!}$$

for α

$$A_{1\alpha}^2 = \sum_{i=2}^{\infty} \frac{e^{-1}}{i!} \times \frac{i^\alpha \times e^{-i}}{\alpha!} + e^{-1} \times \frac{e^{-1}}{\alpha!}$$

$$A_{1\alpha}^2 = \frac{e^{-1}}{\alpha!} S(\alpha) + \frac{e^{-2}}{\alpha!}$$

$$A_{1\alpha}^2 = \frac{e^{-1}}{\alpha!} (S(\alpha) + e^{-1})$$

$$A_{10}^3 = \sum_{i=1}^{\infty} A_{1i}^2 A_{i0}$$

$$= \cancel{e^{-1} S(0)} \sum_{i=1}^{\infty} \frac{e^{-1}}{i!} (S(i) + e^{-1}) e^{-i}$$

4) Yes it also show martingale behaviour since the only change is it amplifies twice in one cycle.

$$\therefore E(x_{n+1} | x_n) = E(x_n)$$

$$\Rightarrow E(x_{n+m} | x_n) = E(x_n)$$

$$\Rightarrow E(x_{2n+2} | x_{2n}) = E(x_{2n})$$

\downarrow next value after two amplifications \downarrow Value after n cycles.